SeparationLogic/ConvexHull/Andrew_Monotone_Chain.v
@@ -1,0 +1,2391 @@
+(* COQ-HEAD *)
+Require Import Coq.ZArith.ZArith.
+Require Import Coq.micromega.Psatz.
+Require Import Coq.Lists.List.
+From ConvexHull Require Import Record_Geo_Point Point_Order Hull_Equiv
+                               Graham_Scan Graham_Scan_M.
+Require Import MonadLib.Monad.
+From MonadLib.StateRelMonad Require StateRelBasic StateRelMonad StateRelHoare.
+Import ListNotations.
+Import Monad MonadNotation.
+Import StateRelBasic StateRelMonad StateRelHoare.
+Local Open Scope Z_scope.
+Local Open Scope monad_scope.
+(* /COQ-HEAD *)
+
+(** Andrew's monotone chain uses the same stack update as [build_hull]:
+    repeatedly pop the stack while the next point would make a non-left turn,
+    then push the point.  The state is the stack with its top at the head. *)
+Definition andrew_scan_stack (l : list point) : list point :=
+  fold_left (fun T p => graham_scan_inc p T) l [].
+
+Definition andrew_chain (l : list point) : list point :=
+  rev (andrew_scan_stack l).
+
+Definition andrew_lower_chain (sorted : list point) : list point :=
+  andrew_chain sorted.
+
+Definition andrew_upper_chain (sorted : list point) : list point :=
+  andrew_chain (rev sorted).
+
+(** [lower] runs from left to right; [upper] runs from right to left.
+    For lists with at least two input points, the last vertex of each chain is
+    duplicated by the other chain, so [removelast] opens both chains before
+    concatenation.
+
+    This is the usual Andrew order.  [Graham_Scan_M.is_convex_hull] uses the
+    opposite directed-edge orientation, so [andrew_merge] below reverses this
+    concrete merge for the specification hull. *)
+Definition andrew_ccw_merge
+    (sorted lower upper : list point) : list point :=
+  match sorted with
+  | [] => []
+  | [_] => sorted
+  | _ => removelast lower ++ removelast upper
+  end.
+
+Definition andrew_merge
+    (sorted lower upper : list point) : list point :=
+  rev (andrew_ccw_merge sorted lower upper).
+
+Definition andrew_hull (sorted : list point) : list point :=
+  andrew_merge
+    sorted
+    (andrew_lower_chain sorted)
+    (andrew_upper_chain sorted).
+
+
+
+
+Definition leftdown (p q : point) : Prop :=
+  x p < x q \/ (x p = x q /\ y p <= y q).
+
+Lemma leftdown_refl : forall p,
+  leftdown p p.
+Proof.
+  unfold leftdown.
+  intros p.
+  right; split; lia.
+Qed.
+
+Lemma leftdown_trans : forall p q r,
+  leftdown p q ->
+  leftdown q r ->
+  leftdown p r.
+Proof.
+  unfold leftdown.
+  intros p q r Hpq Hqr.
+  destruct Hpq as [Hpq | [Hpqx Hpqy]];
+  destruct Hqr as [Hqr | [Hqrx Hqry]]; simpl in *; lia.
+Qed.
+
+Fixpoint point_xy_sorted_from (p : point) (l : list point) : Prop :=
+  match l with
+  | [] => True
+  | q :: rest => leftdown p q /\ point_xy_sorted_from q rest
+  end.
+
+Definition point_xy_sorted (l : list point) : Prop :=
+  match l with
+  | [] => True
+  | p :: rest => point_xy_sorted_from p rest
+  end.
+
+Fixpoint point_xy_rev_sorted_from (p : point) (l : list point) : Prop :=
+  match l with
+  | [] => True
+  | q :: rest => leftdown q p /\ point_xy_rev_sorted_from q rest
+  end.
+
+Definition point_xy_rev_sorted (l : list point) : Prop :=
+  match l with
+  | [] => True
+  | p :: rest => point_xy_rev_sorted_from p rest
+  end.
+
+Lemma point_xy_sorted_from_leftdown_head : forall p l,
+  point_xy_sorted_from p l ->
+  Forall (leftdown p) l.
+Proof.
+  intros p l; revert p.
+  induction l as [| q l IH]; intros p Hsorted; simpl in *.
+  - constructor.
+  - destruct Hsorted as [Hpq Hsorted].
+    constructor; [exact Hpq |].
+    eapply Forall_impl.
+    2: { apply IH. exact Hsorted. }
+    intros r Hqr.
+    eapply leftdown_trans; eauto.
+Qed.
+
+Lemma point_xy_sorted_tail : forall p l,
+  point_xy_sorted_from p l ->
+  point_xy_sorted l.
+Proof.
+  intros p l Hsorted.
+  destruct l as [| q l]; simpl in *; tauto.
+Qed.
+
+Lemma point_xy_rev_sorted_from_leftdown_head : forall p l,
+  point_xy_rev_sorted_from p l ->
+  Forall (fun q => leftdown q p) l.
+Proof.
+  intros p l; revert p.
+  induction l as [| q l IH]; intros p Hsorted; simpl in *.
+  - constructor.
+  - destruct Hsorted as [Hqp Hsorted].
+    constructor; [exact Hqp |].
+    eapply Forall_impl.
+    2: { apply IH. exact Hsorted. }
+    intros r Hrq.
+    exact (leftdown_trans r q p Hrq Hqp).
+Qed.
+
+Lemma point_xy_rev_sorted_tail : forall p l,
+  point_xy_rev_sorted_from p l ->
+  point_xy_rev_sorted l.
+Proof.
+  intros p l Hsorted.
+  destruct l as [| q l]; simpl in *; tauto.
+Qed.
+
+Definition point_list_non_singleton (l : list point) : Prop :=
+  exists p q rest, l = p :: q :: rest.
+
+Definition andrew_hull_geometry (sorted : list point) : Prop :=
+  point_list_non_singleton sorted /\
+  rev_ccw_convex (andrew_hull sorted) /\
+  is_max_hull'_edges (andrew_hull sorted) sorted.
+
+Fixpoint rev_ccw_list (p : point) (l : list point) : Prop :=
+  match l with
+  | q :: l0 => Forall_ccw q p l0 /\ rev_ccw_list p l0
+  | [] => True
+  end.
+
+Lemma graham_scan_inc_rev_consec : forall p T,
+  rev_consec_ccw T ->
+  rev_consec_ccw (graham_scan_inc p T).
+Proof.
+  intros p T.
+  induction T as [| t T IH]; intros Hcon; simpl; try tauto.
+  destruct T as [| s T']; simpl; try tauto.
+  destruct (ccw_dec s t p) as [Hccw | _].
+  - apply rev_consec_ccw_cons_iff.
+    split.
+    + exact Hcon.
+    + intros b c l0 Heq.
+      inversion Heq; subst.
+      apply ccw_cyclicity.
+      exact Hccw.
+  - apply IH.
+    apply rev_consec_ccw_cons_iff in Hcon as [Htail _].
+    exact Htail.
+Qed.
+
+Lemma fold_left_graham_scan_inc_rev_consec : forall l T,
+  rev_consec_ccw T ->
+  rev_consec_ccw
+    (fold_left (fun T p => graham_scan_inc p T) l T).
+Proof.
+  induction l as [| p l IH]; intros T Hcon; simpl.
+  - exact Hcon.
+  - apply IH.
+    apply graham_scan_inc_rev_consec.
+    exact Hcon.
+Qed.
+
+Lemma andrew_scan_stack_rev_consec : forall l,
+  rev_consec_ccw (andrew_scan_stack l).
+Proof.
+  intros l.
+  unfold andrew_scan_stack.
+  apply fold_left_graham_scan_inc_rev_consec.
+  simpl; exact I.
+Qed.
+
+Lemma ccw_leftdown_skip_second : forall p q r s,
+  leftdown p q ->
+  leftdown q r ->
+  leftdown r s ->
+  ccw q p r ->
+  ccw r q s ->
+  ccw r p s.
+Proof.
+  unfold leftdown, x, y, ccw, Record_Geo_Vec.left_than,
+         Record_Geo_Vec.cross_prod, build_vec.
+  simpl; intros; nia.
+Qed.
+
+Lemma ccw_leftdown_extend_head : forall p q r s,
+  leftdown p q ->
+  leftdown q r ->
+  leftdown r s ->
+  ccw q p r ->
+  ccw r q s ->
+  ccw q p s.
+Proof.
+  unfold leftdown, x, y, ccw, Record_Geo_Vec.left_than,
+         Record_Geo_Vec.cross_prod, build_vec.
+  simpl; intros; nia.
+Qed.
+
+Lemma ccw_leftdown_forward_skip_second : forall p q r s,
+  leftdown p q ->
+  leftdown q r ->
+  leftdown r s ->
+  ccw p q r ->
+  ccw q r s ->
+  ccw p r s.
+Proof.
+  unfold leftdown, x, y, ccw, Record_Geo_Vec.left_than,
+         Record_Geo_Vec.cross_prod, build_vec.
+  simpl; intros; nia.
+Qed.
+
+Lemma ccw_leftdown_forward_extend_head : forall p q r s,
+  leftdown p q ->
+  leftdown q r ->
+  leftdown r s ->
+  ccw p q r ->
+  ccw q r s ->
+  ccw p q s.
+Proof.
+  unfold leftdown, x, y, ccw, Record_Geo_Vec.left_than,
+         Record_Geo_Vec.cross_prod, build_vec.
+  simpl; intros; nia.
+Qed.
+
+Lemma ccw_leftdown_rev_forward_skip_second : forall p q r s,
+  leftdown q p ->
+  leftdown r q ->
+  leftdown s r ->
+  ccw p q r ->
+  ccw q r s ->
+  ccw p r s.
+Proof.
+  unfold leftdown, x, y, ccw, Record_Geo_Vec.left_than,
+         Record_Geo_Vec.cross_prod, build_vec.
+  simpl; intros; nia.
+Qed.
+
+Lemma ccw_leftdown_rev_forward_extend_head : forall p q r s,
+  leftdown q p ->
+  leftdown r q ->
+  leftdown s r ->
+  ccw p q r ->
+  ccw q r s ->
+  ccw p q s.
+Proof.
+  unfold leftdown, x, y, ccw, Record_Geo_Vec.left_than,
+         Record_Geo_Vec.cross_prod, build_vec.
+  simpl; intros; nia.
+Qed.
+
+Lemma point_xy_sorted_from_skip_head : forall p q l,
+  leftdown p q ->
+  point_xy_sorted_from q l ->
+  point_xy_sorted_from p l.
+Proof.
+  intros p q l Hpq Hsorted.
+  destruct l as [| r l]; simpl in *; [exact I |].
+  destruct Hsorted as [Hqr Hsorted].
+  split.
+  - eapply leftdown_trans; eauto.
+  - exact Hsorted.
+Qed.
+
+Lemma point_xy_rev_sorted_from_skip_head : forall p q l,
+  leftdown q p ->
+  point_xy_rev_sorted_from q l ->
+  point_xy_rev_sorted_from p l.
+Proof.
+  intros p q l Hqp Hsorted.
+  destruct l as [| r l]; simpl in *; [exact I |].
+  destruct Hsorted as [Hrq Hsorted].
+  split.
+  - eapply leftdown_trans; eauto.
+  - exact Hsorted.
+Qed.
+
+Lemma rev_consec_ccw_skip_second : forall p q l,
+  point_xy_sorted_from p (q :: l) ->
+  rev_consec_ccw (p :: q :: l) ->
+  rev_consec_ccw (p :: l).
+Proof.
+  intros p q l Hsorted Hcon.
+  destruct l as [| r l]; simpl in *; [tauto |].
+  destruct l as [| s l]; simpl in *; [tauto |].
+  destruct Hsorted as [Hpq [Hqr [Hrs _]]].
+  destruct Hcon as [Hqpr [Hrqs Htail]].
+  split.
+  - eapply ccw_leftdown_skip_second; eauto.
+  - exact Htail.
+Qed.
+
+Lemma rev_consec_ccw_skip_third : forall p q r l,
+  point_xy_sorted_from p (q :: r :: l) ->
+  rev_consec_ccw (p :: q :: r :: l) ->
+  rev_consec_ccw (p :: q :: l).
+Proof.
+  intros p q r l Hsorted Hcon.
+  destruct l as [| s l]; simpl in *; [tauto |].
+  destruct Hsorted as [Hpq [Hqr [Hrs Hsorted_s]]].
+  destruct Hcon as [Hqpr Htail].
+  destruct Htail as [Hrqs Htail].
+  split.
+  - eapply ccw_leftdown_extend_head; eauto.
+  - apply (rev_consec_ccw_skip_second q r (s :: l)).
+    + simpl. split; eauto.
+    + simpl. split; eauto.
+Qed.
+
+Lemma xy_rev_consec_ccw_head_forall : forall p q l,
+  point_xy_sorted_from p (q :: l) ->
+  rev_consec_ccw (p :: q :: l) ->
+  Forall_ccw q p l.
+Proof.
+  intros p q l.
+  revert p q.
+  induction l as [| r l IH]; intros p q Hsorted Hcon; simpl in *.
+  - constructor.
+  - rewrite Forall_ccw_cons_iff.
+    pose proof Hsorted as Hsorted_all.
+    pose proof Hcon as Hcon_all.
+    destruct Hsorted as [Hpq Hsorted_q].
+    destruct Hsorted_q as [Hqr Hsorted_r].
+    destruct Hcon as [Hqpr _].
+    split.
+    + exact Hqpr.
+    + apply IH.
+      * simpl.
+        split.
+        -- exact Hpq.
+        -- eapply point_xy_sorted_from_skip_head; eauto.
+      * eapply rev_consec_ccw_skip_third.
+        -- exact Hsorted_all.
+        -- exact Hcon_all.
+Qed.
+
+
+(** Convexity := any three points constitute a clockwise relation *)
+(** convex
+ ** is_convex : consec_ccw + point_xy_sorted -> ccw_list
+*)
+Lemma xy_consec_ccw_to_ccw_list : forall p sorted,
+  point_xy_sorted_from p sorted ->
+  rev_consec_ccw (p :: sorted) ->
+  rev_ccw_list p sorted.
+Proof.
+  intros p sorted.
+  revert p.
+  induction sorted as [| q sorted IH]; intros p Hsorted Hcon; simpl.
+  - exact I.
+  - split.
+    + apply xy_rev_consec_ccw_head_forall; assumption.
+    + destruct Hsorted as [Hpq Hsorted_q].
+      apply IH.
+      * eapply point_xy_sorted_from_skip_head; eauto.
+      * eapply rev_consec_ccw_skip_second.
+        -- simpl. split; eauto.
+        -- exact Hcon.
+Qed.
+
+Lemma consec_ccw_skip_second : forall p q l,
+  point_xy_sorted_from p (q :: l) ->
+  consec_ccw (p :: q :: l) ->
+  consec_ccw (p :: l).
+Proof.
+  intros p q l Hsorted Hcon.
+  destruct l as [| r l]; simpl in *; [tauto |].
+  destruct l as [| s l]; simpl in *; [tauto |].
+  destruct Hsorted as [Hpq [Hqr [Hrs _]]].
+  destruct Hcon as [Hpqr [Hqrs Htail]].
+  split.
+  - eapply ccw_leftdown_forward_skip_second; eauto.
+  - exact Htail.
+Qed.
+
+Lemma consec_ccw_skip_third : forall p q r l,
+  point_xy_sorted_from p (q :: r :: l) ->
+  consec_ccw (p :: q :: r :: l) ->
+  consec_ccw (p :: q :: l).
+Proof.
+  intros p q r l Hsorted Hcon.
+  destruct l as [| s l]; simpl in *; [tauto |].
+  destruct Hsorted as [Hpq [Hqr [Hrs Hsorted_s]]].
+  destruct Hcon as [Hpqr Htail].
+  destruct Htail as [Hqrs Htail].
+  split.
+  - eapply ccw_leftdown_forward_extend_head; eauto.
+  - apply (consec_ccw_skip_second q r (s :: l)).
+    + simpl. split; eauto.
+    + simpl. split; eauto.
+Qed.
+
+Lemma xy_consec_ccw_head_forall : forall p q l,
+  point_xy_sorted_from p (q :: l) ->
+  consec_ccw (p :: q :: l) ->
+  Forall_ccw p q l.
+Proof.
+  intros p q l.
+  revert p q.
+  induction l as [| r l IH]; intros p q Hsorted Hcon; simpl in *.
+  - constructor.
+  - rewrite Forall_ccw_cons_iff.
+    pose proof Hsorted as Hsorted_all.
+    pose proof Hcon as Hcon_all.
+    destruct Hsorted as [Hpq Hsorted_q].
+    destruct Hsorted_q as [Hqr Hsorted_r].
+    destruct Hcon as [Hpqr _].
+    split.
+    + exact Hpqr.
+    + apply IH.
+      * simpl.
+        split.
+        -- exact Hpq.
+        -- eapply point_xy_sorted_from_skip_head; eauto.
+      * eapply consec_ccw_skip_third.
+        -- exact Hsorted_all.
+        -- exact Hcon_all.
+Qed.
+
+Lemma xy_consec_ccw_to_ccw_list_forward : forall p sorted,
+  point_xy_sorted_from p sorted ->
+  consec_ccw (p :: sorted) ->
+  ccw_list p sorted.
+Proof.
+  intros p sorted.
+  revert p.
+  induction sorted as [| q sorted IH]; intros p Hsorted Hcon; simpl.
+  - exact I.
+  - split.
+    + apply xy_consec_ccw_head_forall; assumption.
+    + destruct Hsorted as [Hpq Hsorted_q].
+      apply IH.
+      * eapply point_xy_sorted_from_skip_head; eauto.
+      * eapply consec_ccw_skip_second.
+        -- simpl. split; eauto.
+        -- exact Hcon.
+Qed.
+
+Lemma xy_consec_ccw_to_ccw_convex : forall p sorted,
+  point_xy_sorted_from p sorted ->
+  consec_ccw (p :: sorted) ->
+  ccw_convex (p :: sorted).
+Proof.
+  intros p sorted Hsorted Hcon.
+  apply ccw_convex_spec_simple.
+  - apply xy_consec_ccw_to_ccw_list_forward; assumption.
+  - apply consec_ccw_cons_iff in Hcon.
+    tauto.
+Qed.
+
+Lemma rev_sorted_consec_ccw_skip_second : forall p q l,
+  point_xy_rev_sorted_from p (q :: l) ->
+  consec_ccw (p :: q :: l) ->
+  consec_ccw (p :: l).
+Proof.
+  intros p q l Hsorted Hcon.
+  destruct l as [| r l]; simpl in *; [tauto |].
+  destruct l as [| s l]; simpl in *; [tauto |].
+  destruct Hsorted as [Hqp [Hrq [Hsr _]]].
+  destruct Hcon as [Hpqr [Hqrs Htail]].
+  split.
+  - eapply ccw_leftdown_rev_forward_skip_second; eauto.
+  - exact Htail.
+Qed.
+
+Lemma rev_sorted_consec_ccw_skip_third : forall p q r l,
+  point_xy_rev_sorted_from p (q :: r :: l) ->
+  consec_ccw (p :: q :: r :: l) ->
+  consec_ccw (p :: q :: l).
+Proof.
+  intros p q r l Hsorted Hcon.
+  destruct l as [| s l]; simpl in *; [tauto |].
+  destruct Hsorted as [Hqp [Hrq [Hsr Hsorted_s]]].
+  destruct Hcon as [Hpqr Htail].
+  destruct Htail as [Hqrs Htail].
+  split.
+  - eapply ccw_leftdown_rev_forward_extend_head; eauto.
+  - apply (rev_sorted_consec_ccw_skip_second q r (s :: l)).
+    + simpl. split; eauto.
+    + simpl. split; eauto.
+Qed.
+
+Lemma rev_sorted_consec_ccw_head_forall : forall p q l,
+  point_xy_rev_sorted_from p (q :: l) ->
+  consec_ccw (p :: q :: l) ->
+  Forall_ccw p q l.
+Proof.
+  intros p q l.
+  revert p q.
+  induction l as [| r l IH]; intros p q Hsorted Hcon; simpl in *.
+  - constructor.
+  - rewrite Forall_ccw_cons_iff.
+    pose proof Hsorted as Hsorted_all.
+    pose proof Hcon as Hcon_all.
+    destruct Hsorted as [Hqp Hsorted_q].
+    destruct Hsorted_q as [Hrq Hsorted_r].
+    destruct Hcon as [Hpqr _].
+    split.
+    + exact Hpqr.
+    + apply IH.
+      * simpl.
+        split.
+        -- exact Hqp.
+        -- eapply point_xy_rev_sorted_from_skip_head; eauto.
+      * eapply rev_sorted_consec_ccw_skip_third.
+        -- exact Hsorted_all.
+        -- exact Hcon_all.
+Qed.
+
+Lemma rev_sorted_consec_ccw_to_ccw_list_forward : forall p sorted,
+  point_xy_rev_sorted_from p sorted ->
+  consec_ccw (p :: sorted) ->
+  ccw_list p sorted.
+Proof.
+  intros p sorted.
+  revert p.
+  induction sorted as [| q sorted IH]; intros p Hsorted Hcon; simpl.
+  - exact I.
+  - split.
+    + apply rev_sorted_consec_ccw_head_forall; assumption.
+    + destruct Hsorted as [Hqp Hsorted_q].
+      apply IH.
+      * eapply point_xy_rev_sorted_from_skip_head; eauto.
+      * eapply rev_sorted_consec_ccw_skip_second.
+        -- simpl. split; eauto.
+        -- exact Hcon.
+Qed.
+
+Lemma rev_sorted_consec_ccw_to_ccw_convex : forall p sorted,
+  point_xy_rev_sorted_from p sorted ->
+  consec_ccw (p :: sorted) ->
+  ccw_convex (p :: sorted).
+Proof.
+  intros p sorted Hsorted Hcon.
+  apply ccw_convex_spec_simple.
+  - apply rev_sorted_consec_ccw_to_ccw_list_forward; assumption.
+  - apply consec_ccw_cons_iff in Hcon.
+    tauto.
+Qed.
+
+Lemma point_xy_sorted_from_app_left : forall p l1 l2,
+  point_xy_sorted_from p (l1 ++ l2) ->
+  point_xy_sorted_from p l1.
+Proof.
+  intros p l1.
+  revert p.
+  induction l1 as [| q l1 IH]; intros p l2 Hsorted; simpl in *.
+  - exact I.
+  - destruct Hsorted as [Hpq Hsorted].
+    split.
+    + exact Hpq.
+    + apply IH with (l2 := l2).
+      exact Hsorted.
+Qed.
+
+Lemma point_xy_sorted_app_left : forall l1 l2,
+  point_xy_sorted (l1 ++ l2) ->
+  point_xy_sorted l1.
+Proof.
+  intros l1 l2 Hsorted.
+  destruct l1 as [| p l1]; simpl in *; [exact I |].
+  eapply point_xy_sorted_from_app_left.
+  exact Hsorted.
+Qed.
+
+Lemma point_xy_sorted_from_snoc : forall p l q,
+  point_xy_sorted_from p l ->
+  Forall (fun r => leftdown r q) (p :: l) ->
+  point_xy_sorted_from p (l ++ [q]).
+Proof.
+  intros p l.
+  revert p.
+  induction l as [| r l IH]; intros p q Hsorted Hall; simpl in *.
+  - rewrite Forall_cons_iff in Hall.
+    tauto.
+  - destruct Hsorted as [Hpr Hsorted].
+    rewrite Forall_cons_iff in Hall.
+    destruct Hall as [_ Hall].
+    split.
+    + exact Hpr.
+    + apply IH.
+      * exact Hsorted.
+      * exact Hall.
+Qed.
+
+Lemma point_xy_sorted_snoc : forall l p,
+  point_xy_sorted l ->
+  Forall (fun q => leftdown q p) l ->
+  point_xy_sorted (l ++ [p]).
+Proof.
+  intros l p Hsorted Hall.
+  destruct l as [| q l]; simpl in *.
+  - exact I.
+  - apply point_xy_sorted_from_snoc; assumption.
+Qed.
+
+Lemma point_xy_rev_sorted_from_app_left : forall p l1 l2,
+  point_xy_rev_sorted_from p (l1 ++ l2) ->
+  point_xy_rev_sorted_from p l1.
+Proof.
+  intros p l1.
+  revert p.
+  induction l1 as [| q l1 IH]; intros p l2 Hsorted; simpl in *.
+  - exact I.
+  - destruct Hsorted as [Hqp Hsorted].
+    split.
+    + exact Hqp.
+    + apply IH with (l2 := l2).
+      exact Hsorted.
+Qed.
+
+Lemma point_xy_rev_sorted_app_left : forall l1 l2,
+  point_xy_rev_sorted (l1 ++ l2) ->
+  point_xy_rev_sorted l1.
+Proof.
+  intros l1 l2 Hsorted.
+  destruct l1 as [| p l1]; simpl in *; [exact I |].
+  eapply point_xy_rev_sorted_from_app_left.
+  exact Hsorted.
+Qed.
+
+Lemma point_xy_rev_sorted_from_snoc : forall p l q,
+  point_xy_rev_sorted_from p l ->
+  Forall (fun r => leftdown q r) (p :: l) ->
+  point_xy_rev_sorted_from p (l ++ [q]).
+Proof.
+  intros p l.
+  revert p.
+  induction l as [| r l IH]; intros p q Hsorted Hall; simpl in *.
+  - rewrite Forall_cons_iff in Hall.
+    tauto.
+  - destruct Hsorted as [Hrp Hsorted].
+    rewrite Forall_cons_iff in Hall.
+    destruct Hall as [_ Hall].
+    split.
+    + exact Hrp.
+    + apply IH.
+      * exact Hsorted.
+      * exact Hall.
+Qed.
+
+Lemma point_xy_rev_sorted_snoc : forall l p,
+  point_xy_rev_sorted l ->
+  Forall (fun q => leftdown p q) l ->
+  point_xy_rev_sorted (l ++ [p]).
+Proof.
+  intros l p Hsorted Hall.
+  destruct l as [| q l]; simpl in *.
+  - exact I.
+  - apply point_xy_rev_sorted_from_snoc; assumption.
+Qed.
+
+Lemma point_xy_sorted_rev_tail : forall p T,
+  point_xy_sorted (rev (p :: T)) ->
+  point_xy_sorted (rev T).
+Proof.
+  intros p T Hsorted.
+  simpl in Hsorted.
+  apply (point_xy_sorted_app_left (rev T) [p]).
+  exact Hsorted.
+Qed.
+
+Lemma point_xy_rev_sorted_rev_tail : forall p T,
+  point_xy_rev_sorted (rev (p :: T)) ->
+  point_xy_rev_sorted (rev T).
+Proof.
+  intros p T Hsorted.
+  simpl in Hsorted.
+  apply (point_xy_rev_sorted_app_left (rev T) [p]).
+  exact Hsorted.
+Qed.
+
+Lemma point_xy_sorted_rev_is_rev_sorted : forall l,
+  point_xy_sorted l ->
+  point_xy_rev_sorted (rev l).
+Proof.
+  induction l as [| p l IH]; intros Hsorted; simpl in *.
+  - exact I.
+  - destruct l as [| q l'].
+    + simpl; exact I.
+    + simpl in Hsorted.
+      destruct Hsorted as [Hpq Hsorted_q].
+      simpl.
+      apply point_xy_rev_sorted_snoc.
+      * apply IH.
+        exact Hsorted_q.
+      * change (rev l' ++ [q]) with (rev (q :: l')).
+        apply Forall_rev.
+        apply point_xy_sorted_from_leftdown_head.
+        simpl.
+        split; assumption.
+Qed.
+
+Lemma point_xy_rev_sorted_rev_is_sorted : forall l,
+  point_xy_rev_sorted l ->
+  point_xy_sorted (rev l).
+Proof.
+  induction l as [| p l IH]; intros Hsorted; simpl in *.
+  - exact I.
+  - destruct l as [| q l'].
+    + simpl; exact I.
+    + simpl in Hsorted.
+      destruct Hsorted as [Hqp Hsorted_q].
+      simpl.
+      apply point_xy_sorted_snoc.
+      * apply IH.
+        exact Hsorted_q.
+      * change (rev l' ++ [q]) with (rev (q :: l')).
+        apply Forall_rev.
+        apply point_xy_rev_sorted_from_leftdown_head.
+        simpl.
+        split; assumption.
+Qed.
+
+Lemma graham_scan_inc_Forall : forall (P : point -> Prop) p T,
+  P p ->
+  Forall P T ->
+  Forall P (graham_scan_inc p T).
+Proof.
+  intros P p T.
+  induction T as [| t T IH]; intros Hp HT; simpl in *.
+  - constructor; [exact Hp | constructor].
+  - destruct T as [| s T']; simpl in *.
+    + constructor; [exact Hp | exact HT].
+    + destruct (ccw_dec s t p) as [_ | _].
+      * constructor; [exact Hp | exact HT].
+      * apply IH.
+        -- exact Hp.
+        -- rewrite Forall_cons_iff in HT.
+           exact (proj2 HT).
+Qed.
+
+Lemma graham_scan_inc_in : forall x p T,
+  In x (graham_scan_inc p T) ->
+  x = p \/ In x T.
+Proof.
+  intros x p T.
+  revert p.
+  induction T as [| t T IH]; intros p Hin; simpl in *.
+  - destruct Hin as [Hx | []].
+    subst p; left; reflexivity.
+  - destruct T as [| s T']; simpl in *.
+    + destruct Hin as [Hx | Hin].
+      * subst p; left; reflexivity.
+      * right; simpl; exact Hin.
+    + destruct (ccw_dec s t p) as [_ | _].
+      * destruct Hin as [Hx | Hin].
+        -- subst p; left; reflexivity.
+        -- right; simpl; exact Hin.
+      * specialize (IH p Hin) as [Hx | Hin_tail].
+        -- left; exact Hx.
+        -- right; simpl; right; exact Hin_tail.
+Qed.
+
+Lemma fold_left_graham_scan_inc_in : forall x l T,
+  In x (fold_left (fun T p => graham_scan_inc p T) l T) ->
+  In x l \/ In x T.
+Proof.
+  intros x l.
+  induction l as [| p l IH]; intros T Hin; simpl in *.
+  - right.
+    exact Hin.
+  - specialize (IH (graham_scan_inc p T) Hin) as [Hin_l | Hin_inc].
+    + left.
+      simpl; right.
+      exact Hin_l.
+    + apply graham_scan_inc_in in Hin_inc as [Hx | Hin_T].
+      * subst x.
+        left.
+        simpl; left; reflexivity.
+      * right.
+        exact Hin_T.
+Qed.
+
+Lemma andrew_scan_stack_in : forall x l,
+  In x (andrew_scan_stack l) ->
+  In x l.
+Proof.
+  intros x l Hin.
+  unfold andrew_scan_stack in Hin.
+  apply fold_left_graham_scan_inc_in in Hin as [Hin | Hin].
+  - exact Hin.
+  - contradiction.
+Qed.
+
+Lemma andrew_chain_in : forall x l,
+  In x (andrew_chain l) ->
+  In x l.
+Proof.
+  intros x l Hin.
+  unfold andrew_chain in Hin.
+  apply andrew_scan_stack_in.
+  rewrite in_rev.
+  exact Hin.
+Qed.
+
+Lemma graham_scan_inc_preserves_sorted_chain : forall p T,
+  Forall (fun q => leftdown q p) T ->
+  point_xy_sorted (rev T) ->
+  point_xy_sorted (rev (graham_scan_inc p T)).
+Proof.
+  intros p T.
+  induction T as [| t T IH]; intros Hall Hsorted; simpl in *.
+  - simpl.
+    exact I.
+  - destruct T as [| s T']; simpl in *.
+    + rewrite Forall_cons_iff in Hall.
+      destruct Hall as [Htp _].
+      simpl.
+      split; [exact Htp | exact I].
+    + rewrite Forall_cons_iff in Hall.
+      destruct Hall as [Htp Hall].
+      destruct (ccw_dec s t p) as [_ | _].
+      * simpl.
+        apply point_xy_sorted_snoc.
+        -- exact Hsorted.
+        -- change ((rev T' ++ [s]) ++ [t])
+             with (rev (t :: s :: T')).
+           apply Forall_rev.
+           constructor; assumption.
+      * apply IH.
+        -- exact Hall.
+        -- change (rev T' ++ [s]) with (rev (s :: T')).
+           apply point_xy_sorted_rev_tail with (p := t).
+           exact Hsorted.
+Qed.
+
+Lemma graham_scan_inc_Forall_leftdown_next : forall p q T,
+  Forall (fun r => leftdown r p) T ->
+  leftdown p q ->
+  Forall (fun r => leftdown r q) (graham_scan_inc p T).
+Proof.
+  intros p q T Hall Hpq.
+  apply graham_scan_inc_Forall.
+  - exact Hpq.
+  - eapply Forall_impl.
+    2: exact Hall.
+    intros r Hrp.
+    exact (leftdown_trans r p q Hrp Hpq).
+Qed.
+
+Lemma graham_scan_inc_preserves_rev_sorted_chain : forall p T,
+  Forall (fun q => leftdown p q) T ->
+  point_xy_rev_sorted (rev T) ->
+  point_xy_rev_sorted (rev (graham_scan_inc p T)).
+Proof.
+  intros p T.
+  induction T as [| t T IH]; intros Hall Hsorted; simpl in *.
+  - simpl.
+    exact I.
+  - destruct T as [| s T']; simpl in *.
+    + rewrite Forall_cons_iff in Hall.
+      destruct Hall as [Hpt _].
+      simpl.
+      split; [exact Hpt | exact I].
+    + rewrite Forall_cons_iff in Hall.
+      destruct Hall as [Hpt Hall].
+      destruct (ccw_dec s t p) as [_ | _].
+      * simpl.
+        apply point_xy_rev_sorted_snoc.
+        -- exact Hsorted.
+        -- change ((rev T' ++ [s]) ++ [t])
+             with (rev (t :: s :: T')).
+           apply Forall_rev.
+           constructor; assumption.
+      * apply IH.
+        -- exact Hall.
+        -- change (rev T' ++ [s]) with (rev (s :: T')).
+           apply point_xy_rev_sorted_rev_tail with (p := t).
+           exact Hsorted.
+Qed.
+
+Lemma graham_scan_inc_Forall_leftdown_prev : forall p q T,
+  Forall (fun r => leftdown p r) T ->
+  leftdown q p ->
+  Forall (fun r => leftdown q r) (graham_scan_inc p T).
+Proof.
+  intros p q T Hall Hqp.
+  apply graham_scan_inc_Forall.
+  - exact Hqp.
+  - eapply Forall_impl.
+    2: exact Hall.
+    intros r Hpr.
+    exact (leftdown_trans q p r Hqp Hpr).
+Qed.
+
+Lemma fold_left_graham_scan_inc_sorted_chain : forall l T,
+  point_xy_sorted l ->
+  point_xy_sorted (rev T) ->
+  (match l with
+   | [] => True
+   | p :: _ => Forall (fun q => leftdown q p) T
+   end) ->
+  point_xy_sorted (rev (fold_left (fun T p => graham_scan_inc p T) l T)).
+Proof.
+  induction l as [| p l IH]; intros T Hsorted_l Hsorted_T Hall; simpl in *.
+  - exact Hsorted_T.
+  - assert (Hsorted_inc :
+      point_xy_sorted (rev (graham_scan_inc p T))).
+    {
+      apply graham_scan_inc_preserves_sorted_chain; assumption.
+    }
+    destruct l as [| q l'].
+    + apply IH; simpl; exact I || exact Hsorted_inc.
+    + destruct Hsorted_l as [Hpq Hsorted_q].
+      apply IH.
+      * exact Hsorted_q.
+      * exact Hsorted_inc.
+      * apply graham_scan_inc_Forall_leftdown_next; assumption.
+Qed.
+
+Lemma fold_left_graham_scan_inc_rev_sorted_chain : forall l T,
+  point_xy_rev_sorted l ->
+  point_xy_rev_sorted (rev T) ->
+  (match l with
+   | [] => True
+   | p :: _ => Forall (fun q => leftdown p q) T
+   end) ->
+  point_xy_rev_sorted (rev (fold_left (fun T p => graham_scan_inc p T) l T)).
+Proof.
+  induction l as [| p l IH]; intros T Hsorted_l Hsorted_T Hall; simpl in *.
+  - exact Hsorted_T.
+  - assert (Hsorted_inc :
+      point_xy_rev_sorted (rev (graham_scan_inc p T))).
+    {
+      apply graham_scan_inc_preserves_rev_sorted_chain; assumption.
+    }
+    destruct l as [| q l'].
+    + apply IH; simpl; exact I || exact Hsorted_inc.
+    + destruct Hsorted_l as [Hqp Hsorted_q].
+      apply IH.
+      * exact Hsorted_q.
+      * exact Hsorted_inc.
+      * apply graham_scan_inc_Forall_leftdown_prev; assumption.
+Qed.
+
+Lemma andrew_chain_sorted : forall l,
+  point_xy_sorted l ->
+  point_xy_sorted (andrew_chain l).
+Proof.
+  intros l Hsorted.
+  destruct l as [| p l].
+  - simpl; exact I.
+  - destruct l as [| q l'].
+    + simpl; exact I.
+    + simpl in Hsorted.
+      destruct Hsorted as [Hpq Hsorted_tail].
+      unfold andrew_chain, andrew_scan_stack.
+      change (fold_left (fun T p => graham_scan_inc p T) (p :: q :: l') [])
+        with (fold_left (fun T p => graham_scan_inc p T) (q :: l') [p]).
+      apply fold_left_graham_scan_inc_sorted_chain.
+      * exact Hsorted_tail.
+      * simpl; exact I.
+      * rewrite Forall_cons_iff.
+        split; [exact Hpq | apply Forall_nil].
+Qed.
+
+Lemma andrew_chain_rev_sorted : forall l,
+  point_xy_rev_sorted l ->
+  point_xy_rev_sorted (andrew_chain l).
+Proof.
+  intros l Hsorted.
+  destruct l as [| p l].
+  - simpl; exact I.
+  - destruct l as [| q l'].
+    + simpl; exact I.
+    + simpl in Hsorted.
+      destruct Hsorted as [Hqp Hsorted_tail].
+      unfold andrew_chain, andrew_scan_stack.
+      change (fold_left (fun T p => graham_scan_inc p T) (p :: q :: l') [])
+        with (fold_left (fun T p => graham_scan_inc p T) (q :: l') [p]).
+      apply fold_left_graham_scan_inc_rev_sorted_chain.
+      * exact Hsorted_tail.
+      * simpl; exact I.
+      * rewrite Forall_cons_iff.
+        split; [exact Hqp | apply Forall_nil].
+Qed.
+
+Lemma andrew_chain_consec_ccw : forall l,
+  consec_ccw (andrew_chain l).
+Proof.
+  intros l.
+  unfold andrew_chain.
+  apply gs_rev_consec_ccw_rev_consec.
+  apply andrew_scan_stack_rev_consec.
+Qed.
+
+Lemma andrew_chain_ccw_convex : forall l,
+  point_xy_sorted l ->
+  ccw_convex (andrew_chain l).
+Proof.
+  intros l Hsorted.
+  pose proof (andrew_chain_sorted l Hsorted) as Hchain_sorted.
+  pose proof (andrew_chain_consec_ccw l) as Hchain_consec.
+  destruct (andrew_chain l) as [| p chain] eqn:Hchain; simpl.
+  - exact I.
+  - apply xy_consec_ccw_to_ccw_convex.
+    + exact Hchain_sorted.
+    + exact Hchain_consec.
+Qed.
+
+Lemma andrew_chain_rev_ccw_convex : forall l,
+  point_xy_rev_sorted l ->
+  ccw_convex (andrew_chain l).
+Proof.
+  intros l Hsorted.
+  pose proof (andrew_chain_rev_sorted l Hsorted) as Hchain_sorted.
+  pose proof (andrew_chain_consec_ccw l) as Hchain_consec.
+  destruct (andrew_chain l) as [| p chain] eqn:Hchain; simpl.
+  - exact I.
+  - apply rev_sorted_consec_ccw_to_ccw_convex.
+    + exact Hchain_sorted.
+    + exact Hchain_consec.
+Qed.
+
+Lemma andrew_lower_chain_ccw_convex : forall sorted,
+  point_xy_sorted sorted ->
+  ccw_convex (andrew_lower_chain sorted).
+Proof.
+  intros sorted Hsorted.
+  unfold andrew_lower_chain.
+  apply andrew_chain_ccw_convex.
+  exact Hsorted.
+Qed.
+
+Lemma andrew_upper_chain_ccw_convex : forall sorted,
+  point_xy_sorted sorted ->
+  ccw_convex (andrew_upper_chain sorted).
+Proof.
+  intros sorted Hsorted.
+  unfold andrew_upper_chain.
+  apply andrew_chain_rev_ccw_convex.
+  apply point_xy_sorted_rev_is_rev_sorted.
+  exact Hsorted.
+Qed.
+
+Lemma point_xy_sorted_all_leftdown_last : forall first middle last,
+  point_xy_sorted (first :: (middle ++ [last])) ->
+  Forall (fun q => leftdown q last) (first :: middle ++ [last]).
+Proof.
+  intros first middle.
+  revert first.
+  induction middle as [| q middle IH]; intros first last Hsorted; simpl in *.
+  - destruct Hsorted as [Hfl _].
+    constructor; [exact Hfl |].
+    constructor; [apply leftdown_refl | constructor].
+  - destruct Hsorted as [Hfq Hsorted_q].
+    specialize (IH q last Hsorted_q) as Hall_tail.
+    rewrite Forall_cons_iff in Hall_tail.
+    destruct Hall_tail as [Hql Hall_tail].
+    constructor.
+    + exact (leftdown_trans first q last Hfq Hql).
+    + constructor; [exact Hql | exact Hall_tail].
+Qed.
+
+Lemma point_xy_sorted_middle_between : forall first middle last,
+  point_xy_sorted (first :: (middle ++ [last])) ->
+  Forall (fun q => leftdown first q /\ leftdown q last) middle.
+Proof.
+  intros first middle last Hsorted.
+  assert (Hfirst : Forall (leftdown first) middle).
+  {
+    simpl in Hsorted.
+    apply point_xy_sorted_from_leftdown_head in Hsorted.
+    rewrite Forall_app in Hsorted.
+    tauto.
+  }
+  assert (Hlast : Forall (fun q => leftdown q last) middle).
+  {
+    pose proof (point_xy_sorted_all_leftdown_last first middle last Hsorted)
+      as Hall.
+    rewrite Forall_cons_iff in Hall.
+    destruct Hall as [_ Hall].
+    rewrite Forall_app in Hall.
+    tauto.
+  }
+  rewrite Forall_forall in *.
+  intros q Hq.
+  split; [apply Hfirst | apply Hlast]; exact Hq.
+Qed.
+
+Lemma point_xy_rev_sorted_middle_between : forall first middle last,
+  point_xy_rev_sorted (last :: (middle ++ [first])) ->
+  Forall (fun q => leftdown first q /\ leftdown q last) middle.
+Proof.
+  intros first middle last Hsorted.
+  pose proof (point_xy_rev_sorted_rev_is_sorted
+                (last :: (middle ++ [first])) Hsorted) as Hrev_sorted.
+  simpl in Hrev_sorted.
+  rewrite rev_app_distr in Hrev_sorted.
+  simpl in Hrev_sorted.
+  change (first :: rev middle ++ [last]) with
+    (first :: (rev middle ++ [last])) in Hrev_sorted.
+  pose proof (point_xy_sorted_middle_between first (rev middle) last
+                Hrev_sorted) as Hbetween_rev.
+  rewrite Forall_forall in *.
+  intros q Hq.
+  apply Hbetween_rev.
+  rewrite <- in_rev.
+  exact Hq.
+Qed.
+
+Lemma ccw_anchor_between_trans : forall first q last r,
+  leftdown first q ->
+  leftdown q last ->
+  leftdown first r ->
+  leftdown r last ->
+  ccw first q last ->
+  ccw first last r ->
+  ccw first q r.
+Proof.
+  unfold leftdown, x, y, ccw, Record_Geo_Vec.left_than,
+         Record_Geo_Vec.cross_prod, build_vec.
+  simpl; intros; nia.
+Qed.
+
+Lemma ccw_lower_last_upper : forall first q last r,
+  leftdown first q ->
+  leftdown q last ->
+  leftdown first r ->
+  leftdown r last ->
+  ccw first q last ->
+  ccw first last r ->
+  ccw q last r.
+Proof.
+  unfold leftdown, x, y, ccw, Record_Geo_Vec.left_than,
+         Record_Geo_Vec.cross_prod, build_vec.
+  simpl; intros; nia.
+Qed.
+
+Lemma consec_ccw_append_shared :
+  forall prefix last suffix,
+  consec_ccw (prefix ++ [last]) ->
+  consec_ccw (last :: suffix) ->
+  (forall pre prev u rest,
+      prefix = pre ++ [prev] ->
+      suffix = u :: rest ->
+      ccw prev last u) ->
+  consec_ccw (prefix ++ last :: suffix).
+Proof.
+  induction prefix as [| a prefix IH]; intros last suffix Hprefix Hsuffix Hbridge.
+  - simpl.
+    exact Hsuffix.
+  - simpl in *.
+    apply consec_ccw_cons_iff.
+    split.
+    + apply IH.
+      * apply consec_ccw_cons_iff in Hprefix.
+        tauto.
+      * exact Hsuffix.
+      * intros pre prev u rest Hpre Hsuf.
+        apply (Hbridge (a :: pre) prev u rest).
+        -- simpl. rewrite Hpre. reflexivity.
+        -- exact Hsuf.
+    + intros b c l0 Htail.
+      apply consec_ccw_cons_iff in Hprefix as [_ Hhead].
+      destruct prefix as [| b0 prefix'].
+      * simpl in Htail.
+        destruct suffix as [| u suffix']; [discriminate |].
+        pose proof (Hbridge [] a u suffix' eq_refl eq_refl) as Hccw.
+        inversion Htail; subst.
+        exact Hccw.
+      * destruct prefix' as [| c0 prefix''].
+        -- inversion Htail; subst.
+           apply (Hhead b c []).
+           reflexivity.
+        -- inversion Htail; subst.
+           apply (Hhead b c (prefix'' ++ [last])).
+           reflexivity.
+Qed.
+
+Lemma andrew_hull_convex_from_ccw_merge :
+  forall sorted lower upper,
+  ccw_convex (andrew_ccw_merge sorted lower upper) ->
+  rev_ccw_convex (andrew_merge sorted lower upper).
+Proof.
+  intros sorted lower upper Hconv.
+  unfold andrew_merge.
+  apply gs_ccw_convex_rev_to_rev_ccw_convex.
+  rewrite rev_involutive.
+  exact Hconv.
+Qed.
+
+Lemma andrew_hull_max_singleton_counterexample : forall p,
+  point_xy_sorted [p] /\
+  ~ is_max_hull'_edges (andrew_hull [p]) [p].
+Proof.
+  intros p.
+  split.
+  - simpl; exact I.
+  - simpl.
+    unfold is_max_hull'_edges.
+    rewrite Forall_cons_iff.
+    tauto.
+Qed.
+
+
+(** Maximality := contain all points *)
+Lemma graham_scan_inc_preserves_bottom : forall p stack bottom,
+  exists stack',
+    graham_scan_inc p (stack ++ [bottom]) = stack' ++ [bottom].
+Proof.
+  intros p stack.
+  induction stack as [| a stack IH]; intros bottom.
+  - simpl.
+    exists [p].
+    reflexivity.
+  - destruct stack as [| b stack']; simpl.
+    + destruct (ccw_dec bottom a p) as [_ | _].
+      * exists [p; a].
+        reflexivity.
+      * exists [p].
+        reflexivity.
+    + destruct (ccw_dec b a p) as [_ | _].
+      * exists (p :: a :: b :: stack').
+        reflexivity.
+      * apply IH.
+Qed.
+
+Lemma graham_scan_inc_preserves_bottom_with_head : forall p stack bottom,
+  exists stack',
+    graham_scan_inc p (stack ++ [bottom]) = p :: stack' ++ [bottom].
+Proof.
+  intros p stack.
+  induction stack as [| a stack IH]; intros bottom.
+  - simpl.
+    exists [].
+    reflexivity.
+  - destruct stack as [| b stack']; simpl.
+    + destruct (ccw_dec bottom a p) as [_ | _].
+      * exists [a].
+        reflexivity.
+      * exists [].
+        reflexivity.
+    + destruct (ccw_dec b a p) as [_ | _].
+      * exists (a :: b :: stack').
+        reflexivity.
+      * apply IH.
+Qed.
+
+Lemma fold_left_graham_scan_inc_preserves_bottom : forall l stack bottom,
+  (exists stack', stack = stack' ++ [bottom]) ->
+  exists stack',
+    fold_left (fun T p => graham_scan_inc p T) l stack =
+      stack' ++ [bottom].
+Proof.
+  induction l as [| p l IH]; intros stack bottom [stack' Hstack].
+  - exists stack'.
+    exact Hstack.
+  - simpl.
+    apply IH.
+    subst stack.
+    apply graham_scan_inc_preserves_bottom.
+Qed.
+
+Lemma andrew_scan_stack_preserves_first : forall p l,
+  exists stack',
+    andrew_scan_stack (p :: l) = stack' ++ [p].
+Proof.
+  intros p l.
+  unfold andrew_scan_stack.
+  simpl.
+  apply fold_left_graham_scan_inc_preserves_bottom.
+  exists [].
+  reflexivity.
+Qed.
+
+Lemma graham_scan_inc_has_head : forall p stack,
+  exists stack',
+    graham_scan_inc p stack = p :: stack'.
+Proof.
+  intros p stack.
+  induction stack as [| a stack IH]; simpl.
+  - exists [].
+    reflexivity.
+  - destruct stack as [| b stack']; simpl.
+    + exists [a].
+      reflexivity.
+    + destruct (ccw_dec b a p) as [_ | _].
+      * exists (a :: b :: stack').
+        reflexivity.
+      * apply IH.
+Qed.
+
+Lemma andrew_scan_stack_has_last_head : forall l p,
+  exists stack',
+    andrew_scan_stack (l ++ [p]) = p :: stack'.
+Proof.
+  intros l p.
+  unfold andrew_scan_stack.
+  rewrite fold_left_app.
+  simpl.
+  apply graham_scan_inc_has_head.
+Qed.
+
+Lemma andrew_chain_starts_first : forall p l,
+  exists chain',
+    andrew_chain (p :: l) = p :: chain'.
+Proof.
+  intros p l.
+  unfold andrew_chain.
+  destruct (andrew_scan_stack_preserves_first p l) as [stack' Hstack].
+  rewrite Hstack.
+  rewrite rev_app_distr.
+  simpl.
+  exists (rev stack').
+  reflexivity.
+Qed.
+
+Lemma andrew_chain_ends_last : forall l p,
+  exists chain',
+    andrew_chain (l ++ [p]) = chain' ++ [p].
+Proof.
+  intros l p.
+  unfold andrew_chain.
+  destruct (andrew_scan_stack_has_last_head l p) as [stack' Hstack].
+  rewrite Hstack.
+  simpl.
+  exists (rev stack').
+  reflexivity.
+Qed.
+
+Lemma andrew_scan_stack_endpoints : forall first middle last,
+  exists stack_mid,
+    andrew_scan_stack (first :: (middle ++ [last])) =
+      last :: stack_mid ++ [first].
+Proof.
+  intros first middle last.
+  destruct (andrew_scan_stack_preserves_first first middle) as [stack' Hstack].
+  unfold andrew_scan_stack in *.
+  simpl in Hstack.
+  change (first :: (middle ++ [last])) with ((first :: middle) ++ [last]).
+  rewrite fold_left_app.
+  simpl.
+  rewrite Hstack.
+  apply graham_scan_inc_preserves_bottom_with_head.
+Qed.
+
+Lemma point_list_non_singleton_first_last : forall sorted,
+  point_list_non_singleton sorted ->
+  exists first middle last,
+    sorted = first :: (middle ++ [last]).
+Proof.
+  intros sorted [first [second [rest Hsorted]]].
+  subst sorted.
+  revert first second.
+  induction rest as [| a rest IH]; intros first second.
+  - exists first, [], second.
+    reflexivity.
+  - specialize (IH second a) as [head [middle [last Hshape]]].
+    exists first, (head :: middle), last.
+    rewrite Hshape.
+    reflexivity.
+Qed.
+
+Lemma andrew_lower_chain_endpoints : forall first middle last,
+  exists lower_mid,
+    andrew_lower_chain (first :: (middle ++ [last])) =
+      first :: (lower_mid ++ [last]).
+Proof.
+  intros first middle last.
+  unfold andrew_lower_chain, andrew_chain.
+  destruct (andrew_scan_stack_endpoints first middle last) as [stack_mid Hstack].
+  rewrite Hstack.
+  simpl.
+  rewrite rev_app_distr.
+  simpl.
+  exists (rev stack_mid).
+  reflexivity.
+Qed.
+
+Lemma andrew_upper_chain_endpoints : forall first middle last,
+  exists upper_mid,
+    andrew_upper_chain (first :: (middle ++ [last])) =
+      last :: (upper_mid ++ [first]).
+Proof.
+  intros first middle last.
+  unfold andrew_upper_chain, andrew_chain.
+  replace (rev (first :: (middle ++ [last])))
+    with (last :: (rev middle ++ [first])).
+  2: {
+    simpl.
+    rewrite rev_app_distr.
+    simpl.
+    reflexivity.
+  }
+  destruct (andrew_scan_stack_endpoints last (rev middle) first)
+    as [stack_mid Hstack].
+  rewrite Hstack.
+  simpl.
+  rewrite rev_app_distr.
+  simpl.
+  exists (rev stack_mid).
+  reflexivity.
+Qed.
+
+Lemma removelast_snoc : forall {A : Type} (l : list A) x,
+  removelast (l ++ [x]) = l.
+Proof.
+  intros A l.
+  induction l as [| a l IH]; intros x; simpl.
+  - reflexivity.
+  - destruct l as [| b l']; simpl.
+    + reflexivity.
+    + f_equal.
+      apply IH.
+Qed.
+
+Lemma andrew_ccw_merge_endpoints :
+  forall sorted first middle last lower upper lower_mid upper_mid,
+  sorted = first :: (middle ++ [last]) ->
+  lower = first :: (lower_mid ++ [last]) ->
+  upper = last :: (upper_mid ++ [first]) ->
+  andrew_ccw_merge sorted lower upper =
+    first :: (lower_mid ++ last :: upper_mid).
+Proof.
+  intros sorted first middle last lower upper lower_mid upper_mid
+    Hsorted Hlower Hupper.
+  subst sorted lower upper.
+  unfold andrew_ccw_merge.
+  destruct middle as [| m middle].
+  - change (removelast (first :: (lower_mid ++ [last])) ++
+            removelast (last :: (upper_mid ++ [first])) =
+            first :: (lower_mid ++ last :: upper_mid)).
+    change (first :: (lower_mid ++ [last]))
+      with ((first :: lower_mid) ++ [last]).
+    change (last :: (upper_mid ++ [first]))
+      with ((last :: upper_mid) ++ [first]).
+    rewrite !removelast_snoc.
+    reflexivity.
+  - change (removelast (first :: (lower_mid ++ [last])) ++
+            removelast (last :: (upper_mid ++ [first])) =
+            first :: (lower_mid ++ last :: upper_mid)).
+    change (first :: (lower_mid ++ [last]))
+      with ((first :: lower_mid) ++ [last]).
+    change (last :: (upper_mid ++ [first]))
+      with ((last :: upper_mid) ++ [first]).
+    rewrite !removelast_snoc.
+    reflexivity.
+Qed.
+
+Lemma point_in_hull_edges_two_points_endpoints : forall p q,
+  point_in_hull_edges p [q; p] /\
+  point_in_hull_edges q [q; p].
+Proof.
+  intros p q.
+  simpl.
+  split; split;
+    unfold colinear, at_mid, Record_Geo_Vec.parallel,
+           Record_Geo_Vec.backward_or_perp,
+           Record_Geo_Vec.cross_prod, Record_Geo_Vec.dot_prod, build_vec;
+    simpl; nia.
+Qed.
+
+Lemma andrew_hull_max_two_points : forall p q,
+  is_max_hull'_edges (andrew_hull [p; q]) [p; q].
+Proof.
+  intros p q.
+  simpl.
+  unfold is_max_hull'_edges.
+  rewrite !Forall_cons_iff.
+  rewrite Forall_nil_iff.
+  pose proof point_in_hull_edges_two_points_endpoints p q as [Hp Hq].
+  tauto.
+Qed.
+
+Lemma andrew_hull_merge_shape : forall first middle last,
+  exists lower_mid upper_mid,
+    andrew_hull (first :: (middle ++ [last])) =
+      rev (first :: (lower_mid ++ last :: upper_mid)) /\
+    andrew_lower_chain (first :: (middle ++ [last])) =
+      first :: (lower_mid ++ [last]) /\
+    andrew_upper_chain (first :: (middle ++ [last])) =
+      last :: (upper_mid ++ [first]).
+Proof.
+  intros first middle last.
+  destruct (andrew_lower_chain_endpoints first middle last)
+    as [lower_mid Hlower].
+  destruct (andrew_upper_chain_endpoints first middle last)
+    as [upper_mid Hupper].
+  exists lower_mid, upper_mid.
+  assert (Hmerge :
+    andrew_ccw_merge
+      (first :: (middle ++ [last]))
+      (andrew_lower_chain (first :: (middle ++ [last])))
+      (andrew_upper_chain (first :: (middle ++ [last]))) =
+      first :: (lower_mid ++ last :: upper_mid)).
+  {
+    eapply andrew_ccw_merge_endpoints; eauto.
+  }
+  split.
+  - unfold andrew_hull, andrew_merge.
+    rewrite Hmerge.
+    reflexivity.
+  - split; assumption.
+Qed.
+
+Theorem andrew_hull_convex : forall sorted,
+  point_xy_sorted sorted ->
+  rev_ccw_convex (andrew_hull sorted).
+Proof.
+  intros sorted Hsorted.
+  destruct sorted as [| p sorted'].
+  - simpl.
+    apply gs_ccw_convex_rev_to_rev_ccw_convex.
+    simpl; exact I.
+  - destruct sorted' as [| q rest].
+    + simpl.
+      apply gs_ccw_convex_rev_to_rev_ccw_convex.
+      simpl; tauto.
+    + assert (Hnonsingleton : point_list_non_singleton (p :: q :: rest)).
+      {
+        exists p, q, rest.
+        reflexivity.
+      }
+      destruct (point_list_non_singleton_first_last
+                  (p :: q :: rest) Hnonsingleton)
+        as [first [middle [last Hshape]]].
+      rewrite Hshape in Hsorted |- *.
+      destruct (andrew_lower_chain_endpoints first middle last)
+        as [lower_mid Hlower].
+      destruct (andrew_upper_chain_endpoints first middle last)
+        as [upper_mid Hupper].
+      unfold andrew_hull.
+      apply andrew_hull_convex_from_ccw_merge.
+      assert (Hmerge :
+        andrew_ccw_merge
+          (first :: middle ++ [last])
+          (andrew_lower_chain (first :: middle ++ [last]))
+          (andrew_upper_chain (first :: middle ++ [last])) =
+          first :: lower_mid ++ last :: upper_mid).
+      {
+        eapply andrew_ccw_merge_endpoints; eauto.
+      }
+      rewrite Hmerge.
+      pose proof (andrew_lower_chain_ccw_convex
+                    (first :: middle ++ [last]) Hsorted) as Hlower_conv.
+      pose proof (andrew_upper_chain_ccw_convex
+                    (first :: middle ++ [last]) Hsorted) as Hupper_conv.
+      pose proof (andrew_chain_sorted
+                    (first :: middle ++ [last]) Hsorted) as Hlower_sorted.
+      unfold andrew_chain in Hlower_sorted.
+      fold (andrew_chain (first :: middle ++ [last])) in Hlower_sorted.
+      change (andrew_chain (first :: middle ++ [last]))
+        with (andrew_lower_chain (first :: middle ++ [last]))
+        in Hlower_sorted.
+      rewrite Hlower in Hlower_sorted.
+      pose proof (andrew_chain_rev_sorted
+                    (rev (first :: middle ++ [last]))
+                    (point_xy_sorted_rev_is_rev_sorted
+                       (first :: middle ++ [last]) Hsorted))
+        as Hupper_sorted.
+      change (andrew_chain (rev (first :: middle ++ [last])))
+        with (andrew_upper_chain (first :: middle ++ [last]))
+        in Hupper_sorted.
+      rewrite Hupper in Hupper_sorted.
+      rewrite Hlower in Hlower_conv.
+      rewrite Hupper in Hupper_conv.
+      pose proof (point_xy_sorted_middle_between
+                    first lower_mid last Hlower_sorted) as Hlower_between.
+      pose proof (point_xy_rev_sorted_middle_between
+                    first upper_mid last Hupper_sorted) as Hupper_between.
+      pose proof (andrew_chain_consec_ccw
+                    (first :: middle ++ [last])) as Hlower_consec.
+      change (andrew_chain (first :: middle ++ [last]))
+        with (andrew_lower_chain (first :: middle ++ [last]))
+        in Hlower_consec.
+      rewrite Hlower in Hlower_consec.
+      pose proof (andrew_chain_consec_ccw
+                    (rev (first :: middle ++ [last]))) as Hupper_consec.
+      change (andrew_chain (rev (first :: middle ++ [last])))
+        with (andrew_upper_chain (first :: middle ++ [last]))
+        in Hupper_consec.
+      rewrite Hupper in Hupper_consec.
+      pose proof (ccw_convex_app_comm (last :: upper_mid) [first]
+                    Hupper_conv) as Hupper_rot.
+      simpl in Hlower_conv.
+      destruct Hlower_conv as [Hlower_list _].
+      simpl in Hupper_rot.
+      destruct Hupper_rot as [Hupper_first_list _].
+      assert (Hlower_first_last :
+        forall q, In q lower_mid -> ccw first q last).
+      {
+        intros a Ha.
+        rewrite ccw_list_app_iff in Hlower_list.
+        destruct Hlower_list as [_ [_ Hcross]].
+        apply Hcross; [exact Ha | simpl; auto].
+      }
+      assert (Hupper_first_last :
+        forall q, In q upper_mid -> ccw first last q).
+      {
+        simpl in Hupper_first_list.
+        destruct Hupper_first_list as [Hforall _].
+        rewrite Forall_ccw_forall in Hforall.
+        intros a Ha.
+        apply Hforall.
+        exact Ha.
+      }
+      apply ccw_convex_spec.
+      * apply g_ccw_ccw_list.
+        apply ccw_list_app_iff.
+        split.
+        -- rewrite ccw_list_app_iff in Hlower_list; tauto.
+        -- split.
+           ++ exact Hupper_first_list.
+           ++ intros a b Ha Hb.
+           destruct Hb as [Hb | Hb].
+           ** subst b.
+              apply Hlower_first_last.
+              exact Ha.
+           ** apply ccw_anchor_between_trans with (last := last).
+              --- rewrite Forall_forall in Hlower_between.
+                 exact (proj1 (Hlower_between a Ha)).
+              --- rewrite Forall_forall in Hlower_between.
+                 exact (proj2 (Hlower_between a Ha)).
+              --- rewrite Forall_forall in Hupper_between.
+                 exact (proj1 (Hupper_between b Hb)).
+              --- rewrite Forall_forall in Hupper_between.
+                 exact (proj2 (Hupper_between b Hb)).
+              --- apply Hlower_first_last.
+                 exact Ha.
+              --- apply Hupper_first_last.
+                 exact Hb.
+      * apply (consec_ccw_append_shared
+                 (first :: lower_mid) last upper_mid).
+        -- exact Hlower_consec.
+        -- apply (consec_ccw_app_inv1 (last :: upper_mid) [first]).
+           change ((last :: upper_mid) ++ [first])
+             with (last :: upper_mid ++ [first]).
+           exact Hupper_consec.
+        -- intros pre prev u tail Hprefix Hsuffix.
+           assert (Hu : In u upper_mid).
+           {
+             rewrite Hsuffix.
+             simpl; auto.
+           }
+           destruct pre as [| a pre'].
+           ++ simpl in Hprefix.
+              inversion Hprefix; subst.
+              apply Hupper_first_last.
+              exact Hu.
+           ++ simpl in Hprefix.
+              inversion Hprefix as [[Hfirst_eq Hmid_eq]].
+              subst a.
+              assert (Hprev : In prev lower_mid).
+              {
+                rewrite Hmid_eq.
+                rewrite in_app_iff.
+                right; simpl; auto.
+              }
+              apply ccw_lower_last_upper with (first := first).
+              ** rewrite Forall_forall in Hlower_between.
+                 exact (proj1 (Hlower_between prev Hprev)).
+              ** rewrite Forall_forall in Hlower_between.
+                 exact (proj2 (Hlower_between prev Hprev)).
+              ** rewrite Forall_forall in Hupper_between.
+                 exact (proj1 (Hupper_between u Hu)).
+              ** rewrite Forall_forall in Hupper_between.
+                 exact (proj2 (Hupper_between u Hu)).
+              ** apply Hlower_first_last.
+                 exact Hprev.
+              ** apply Hupper_first_last.
+                 exact Hu.
+Qed.
+
+Lemma point_in_hull_cons_weak : forall p q p0 T,
+  weak_rev_ccw_list p (p0 :: T) ->
+  point_in_hull q (p :: T) ->
+  point_in_hull q (p :: p0 :: T).
+Proof.
+  intros p q p0 T Hweak Hinh.
+  destruct T as [| a T].
+  - simpl in Hinh.
+    contradiction.
+  - pose proof (proj2 (point_in_hull_cons_iff_weak q p a p0 T Hweak))
+      as Hto.
+    apply Hto.
+    left.
+    exact Hinh.
+Qed.
+
+Lemma is_max_hull'_cons_weak : forall p p0 T L,
+  weak_rev_ccw_list p (p0 :: T) ->
+  is_max_hull' p T L ->
+  is_max_hull' p (p0 :: T) L.
+Proof.
+  intros p p0 T L Hweak Hmax.
+  unfold is_max_hull' in *.
+  rewrite Forall_forall in *.
+  intros q Hq.
+  apply point_in_hull_cons_weak; [exact Hweak |].
+  apply Hmax.
+  exact Hq.
+Qed.
+
+Lemma point_in_tri_snoc_edge_weak : forall p q b a,
+  weak_rev_ccw p b a ->
+  colinear q p b ->
+  at_mid q p b ->
+  point_in_triangle q b a p.
+Proof.
+  intros p q b a Hweak Hcol Hmid.
+  destruct Hweak as [Hstrict | [Hcol_ba Hmid_a]].
+  - rewrite point_in_tri_cyclicity.
+    eapply point_in_tri_col_mid'.
+    + apply ccw_cyclicity_2.
+      exact Hstrict.
+    + exact Hcol.
+    + exact Hmid.
+  - right.
+    unfold colinear, Record_Geo_Vec.parallel,
+           at_mid, Record_Geo_Vec.backward_or_perp,
+           ccw, Record_Geo_Vec.left_than, Record_Geo_Vec.left_equal,
+           Record_Geo_Vec.cross_prod, Record_Geo_Vec.dot_prod, build_vec
+      in *.
+    simpl in *.
+    nia.
+Qed.
+
+Lemma point_in_hull_snoc_weak : forall p q a CH,
+  weak_rev_ccw_list p (CH ++ [a]) ->
+  point_in_hull q (p :: CH) ->
+  point_in_hull q (p :: CH ++ [a]).
+Proof.
+  intros p q a CH.
+  induction CH as [| b CH IH]; intros Hweak Hinh.
+  - simpl in Hinh.
+    contradiction.
+  - destruct CH as [| c CH'].
+    + simpl in *.
+      destruct Hweak as [Hfor _].
+      rewrite Forall_weak_rev_ccw_cons_iff in Hfor.
+      destruct Hfor as [Hba _].
+      destruct Hinh as [Hcol Hmid].
+      left.
+      exact (point_in_tri_snoc_edge_weak p q b a Hba Hcol Hmid).
+    + change (p :: b :: c :: CH' ++ [a])
+        with (p :: b :: (c :: CH' ++ [a])).
+      pose proof (point_in_hull_cons_iff_weak q p c b (CH' ++ [a]) Hweak)
+        as [_ Hto].
+      apply Hto.
+      assert (Hsmall_weak : weak_rev_ccw_list p (b :: c :: CH')).
+      {
+        assert (Hweak' :
+          weak_rev_ccw_list p ((b :: c :: CH') ++ [a] ++ [])).
+        {
+          rewrite app_nil_r.
+          exact Hweak.
+        }
+        pose proof (weak_rev_ccw_list_remove_middle
+                      p (b :: c :: CH') [a] [] Hweak') as Htmp.
+        rewrite app_nil_r in Htmp.
+        exact Htmp.
+      }
+      pose proof (point_in_hull_cons_iff_weak q p c b CH' Hsmall_weak)
+        as [Hfrom _].
+      destruct (Hfrom Hinh) as [Hsmall | Htri].
+      * left.
+        destruct Hweak as [_ Htail_weak].
+        apply (IH Htail_weak Hsmall).
+      * right.
+        exact Htri.
+Qed.
+
+Lemma point_in_hull_last_weak : forall p CH a,
+  weak_rev_ccw_list p (CH ++ [a]) ->
+  point_in_hull a (p :: CH ++ [a]).
+Proof.
+  intros p CH a Hweak.
+  induction CH as [| b CH IH].
+  - simpl.
+    unfold colinear, Record_Geo_Vec.parallel,
+           at_mid, Record_Geo_Vec.backward_or_perp,
+           Record_Geo_Vec.cross_prod, Record_Geo_Vec.dot_prod, build_vec.
+    simpl.
+    split; lia.
+  - change (p :: b :: CH ++ [a]) with (p :: b :: (CH ++ [a])).
+    eapply point_in_hull_cons_weak.
+    + exact Hweak.
+    + apply IH.
+      destruct Hweak as [_ Htail_weak].
+      exact Htail_weak.
+Qed.
+
+Lemma is_max_hull'_snoc_weak : forall p a CH l,
+  weak_rev_ccw_list p (CH ++ [a]) ->
+  is_max_hull' p CH l ->
+  is_max_hull' p (CH ++ [a]) l.
+Proof.
+  intros p a CH l Hweak Hmax.
+  unfold is_max_hull' in *.
+  rewrite Forall_forall in *.
+  intros q Hq.
+  eapply point_in_hull_snoc_weak; eauto.
+Qed.
+
+Lemma is_max_hull'_snoc_self_weak : forall p a CH l,
+  weak_rev_ccw_list p (CH ++ [a]) ->
+  is_max_hull' p CH l ->
+  is_max_hull' p (CH ++ [a]) (l ++ [a]).
+Proof.
+  intros p a CH l Hweak Hmax.
+  unfold is_max_hull' in *.
+  rewrite Forall_app.
+  split.
+  - apply is_max_hull'_snoc_weak; assumption.
+  - apply Forall_cons.
+    + apply point_in_hull_last_weak.
+      exact Hweak.
+    + apply Forall_nil.
+Qed.
+
+Lemma g_ccw_to_g_rev_ccw_rev : forall p q r,
+  g_ccw p r q ->
+  g_rev_ccw p q r.
+Proof.
+  intros p q r H.
+  rewrite g_rev_ccw_iff_g_ccw_rev.
+  exact H.
+Qed.
+
+Lemma g_ccw_list_to_g_rev_ccw_list_rev : forall p l,
+  g_ccw_list p l ->
+  g_rev_ccw_list p (rev l).
+Proof.
+  intros p l.
+  induction l as [| a l IH]; simpl; intros Hccw.
+  - exact I.
+  - destruct Hccw as [Ha Htail].
+    rewrite g_rev_ccw_list_app_iff.
+    repeat split.
+    + apply IH.
+      exact Htail.
+    + unfold g_rev_ccw_list.
+      simpl.
+      repeat constructor.
+    + intros q r Hq Hr.
+      simpl in Hr.
+      destruct Hr as [Hr | []].
+      subst r.
+      rewrite Forall_forall in Ha.
+      apply g_ccw_to_g_rev_ccw_rev.
+      apply Ha.
+      rewrite in_rev.
+      exact Hq.
+Qed.
+
+Lemma leftmost_rev : forall p l,
+  leftmost p l ->
+  leftmost p (rev l).
+Proof.
+  intros p l Hleft.
+  unfold leftmost in *.
+  rewrite Forall_forall in *.
+  intros q Hq.
+  apply Hleft.
+  rewrite in_rev.
+  exact Hq.
+Qed.
+
+Lemma ccw_convex_tail_sort_rev : forall p l,
+  leftmost p l ->
+  ccw_convex (p :: l) ->
+  sort p (rev l).
+Proof.
+  intros p l Hleft Hconv.
+  simpl in Hconv.
+  destruct Hconv as [Hlist _].
+  split.
+  - apply leftmost_rev.
+    exact Hleft.
+  - apply g_ccw_list_to_g_rev_ccw_list_rev.
+    apply g_ccw_ccw_list.
+    exact Hlist.
+Qed.
+
+Lemma rev_consec_ccw_of_consec_rev : forall l,
+  consec_ccw (rev l) ->
+  rev_consec_ccw l.
+Proof.
+  induction l as [| a l IH]; intros Hcon.
+  - simpl; exact I.
+  - rewrite rev_consec_ccw_cons_iff.
+    split.
+    + apply IH.
+      simpl in Hcon.
+      apply (consec_ccw_app_inv1 (rev l) [a]).
+      exact Hcon.
+    + intros b c l0 Hl.
+      subst l.
+      simpl in Hcon.
+      rewrite consec_ccw_snoc_iff in Hcon.
+      destruct Hcon as [_ Hlast].
+      apply ccw_cyclicity.
+      apply (Hlast b c (rev l0)).
+      simpl.
+      rewrite <- app_assoc.
+      reflexivity.
+Qed.
+
+Lemma consec_ccw_rev_rev_consec : forall l,
+  consec_ccw l ->
+  rev_consec_ccw (rev l).
+Proof.
+  intros l Hcon.
+  apply rev_consec_ccw_of_consec_rev.
+  rewrite rev_involutive.
+  exact Hcon.
+Qed.
+
+Lemma ccw_convex_consec_ccw : forall l,
+  ccw_convex l ->
+  consec_ccw l.
+Proof.
+  induction l as [| p l IH]; intros Hconv; simpl.
+  - exact I.
+  - destruct Hconv as [Hlist Htail].
+    split.
+    + destruct l as [| q [| r rest]]; simpl; exact I || idtac.
+      simpl in Hlist.
+      destruct Hlist as [Hfor _].
+      rewrite Forall_ccw_cons_iff in Hfor.
+      exact (proj1 Hfor).
+    + apply IH.
+      exact Htail.
+Qed.
+
+Lemma merged_triangle_max_to_edges : forall first tail base,
+  leftmost first tail ->
+  ccw_convex (first :: tail) ->
+  consec_ccw tail ->
+  is_max_hull' first (rev tail) base ->
+  is_max_hull'_edges (rev (first :: tail)) base.
+Proof.
+  intros first tail base Hleft Hconv Hconsec Hmax.
+  simpl.
+  apply gs_is_max_hull'_edges_rotate1.
+  eapply is_max_hull'_edges_of_max_hull.
+  - apply ccw_convex_tail_sort_rev; assumption.
+  - apply consec_ccw_rev_rev_consec.
+    exact Hconsec.
+  - exact Hmax.
+Qed.
+
+Lemma merged_triangle_max_to_edges_from_convex : forall first tail base,
+  leftmost first tail ->
+  ccw_convex (first :: tail) ->
+  is_max_hull' first (rev tail) base ->
+  is_max_hull'_edges (rev (first :: tail)) base.
+Proof.
+  intros first tail base Hleft Hconv Hmax.
+  apply merged_triangle_max_to_edges.
+  - exact Hleft.
+  - exact Hconv.
+  - pose proof (ccw_convex_consec_ccw (first :: tail) Hconv) as Hconsec.
+    apply consec_ccw_cons_iff in Hconsec as [Htail _].
+    exact Htail.
+  - exact Hmax.
+Qed.
+
+Lemma andrew_ccw_merge_leftmost :
+  forall first middle last lower_mid upper_mid,
+  point_xy_sorted (first :: middle ++ [last]) ->
+  andrew_lower_chain (first :: middle ++ [last]) =
+    first :: lower_mid ++ [last] ->
+  andrew_upper_chain (first :: middle ++ [last]) =
+    last :: upper_mid ++ [first] ->
+  leftmost first (lower_mid ++ last :: upper_mid).
+Proof.
+  intros first middle last lower_mid upper_mid Hsorted Hlower Hupper.
+  assert (Hlower_sorted :
+    point_xy_sorted (first :: lower_mid ++ [last])).
+  {
+    pose proof (andrew_chain_sorted
+                  (first :: middle ++ [last]) Hsorted) as Hchain_sorted.
+    change (andrew_chain (first :: middle ++ [last]))
+      with (andrew_lower_chain (first :: middle ++ [last]))
+      in Hchain_sorted.
+    rewrite Hlower in Hchain_sorted.
+    exact Hchain_sorted.
+  }
+  assert (Hupper_sorted :
+    point_xy_rev_sorted (last :: upper_mid ++ [first])).
+  {
+    pose proof (andrew_chain_rev_sorted
+                  (rev (first :: middle ++ [last]))
+                  (point_xy_sorted_rev_is_rev_sorted
+                     (first :: middle ++ [last]) Hsorted)) as Hchain_sorted.
+    change (andrew_chain (rev (first :: middle ++ [last])))
+      with (andrew_upper_chain (first :: middle ++ [last]))
+      in Hchain_sorted.
+    rewrite Hupper in Hchain_sorted.
+    exact Hchain_sorted.
+  }
+  assert (Hlower_all : Forall (leftdown first) (lower_mid ++ [last])).
+  {
+    simpl in Hlower_sorted.
+    apply point_xy_sorted_from_leftdown_head.
+    exact Hlower_sorted.
+  }
+  pose proof (point_xy_rev_sorted_middle_between
+                first upper_mid last Hupper_sorted) as Hupper_between.
+  unfold leftmost.
+  rewrite Forall_forall.
+  intros q Hq.
+  replace (lower_mid ++ last :: upper_mid)
+    with ((lower_mid ++ [last]) ++ upper_mid) in Hq
+    by (rewrite <- app_assoc; reflexivity).
+  rewrite in_app_iff in Hq.
+  destruct Hq as [Hq | Hq].
+  - rewrite Forall_forall in Hlower_all.
+    exact (Hlower_all q Hq).
+  - rewrite Forall_forall in Hupper_between.
+    exact (proj1 (Hupper_between q Hq)).
+Qed.
+
+Lemma andrew_merged_triangle_max_to_edges :
+  forall first middle last lower_mid upper_mid,
+  point_xy_sorted (first :: middle ++ [last]) ->
+  andrew_lower_chain (first :: middle ++ [last]) =
+    first :: lower_mid ++ [last] ->
+  andrew_upper_chain (first :: middle ++ [last]) =
+    last :: upper_mid ++ [first] ->
+  ccw_convex (first :: lower_mid ++ last :: upper_mid) ->
+  is_max_hull' first (rev (lower_mid ++ last :: upper_mid))
+    (first :: middle ++ [last]) ->
+  is_max_hull'_edges
+    (andrew_hull (first :: middle ++ [last]))
+    (first :: middle ++ [last]).
+Proof.
+  intros first middle last lower_mid upper_mid
+    Hsorted Hlower Hupper Hconv Hmax.
+  unfold andrew_hull, andrew_merge.
+  assert (Hmerge :
+    andrew_ccw_merge
+      (first :: middle ++ [last])
+      (andrew_lower_chain (first :: middle ++ [last]))
+      (andrew_upper_chain (first :: middle ++ [last])) =
+      first :: lower_mid ++ last :: upper_mid).
+  {
+    eapply andrew_ccw_merge_endpoints; eauto.
+  }
+  rewrite Hmerge.
+  apply merged_triangle_max_to_edges_from_convex.
+  - eapply andrew_ccw_merge_leftmost; eauto.
+  - exact Hconv.
+  - exact Hmax.
+Qed.
+
+Lemma weak_rev_ccw_list_app_prefix :
+  forall p prefix suffix,
+  weak_rev_ccw_list p (prefix ++ suffix) ->
+  weak_rev_ccw_list p prefix.
+Proof.
+  intros p prefix suffix Hweak.
+  rewrite weak_rev_ccw_list_app_iff in Hweak.
+  tauto.
+Qed.
+
+Lemma point_in_hull_prepend_many_weak :
+  forall p prefix CH q,
+  weak_rev_ccw_list p (prefix ++ CH) ->
+  point_in_hull q (p :: CH) ->
+  point_in_hull q (p :: prefix ++ CH).
+Proof.
+  intros p prefix.
+  induction prefix as [| a prefix IH]; intros CH q Hweak Hinh.
+  - simpl.
+    exact Hinh.
+  - simpl in Hweak |- *.
+    apply point_in_hull_cons_weak.
+    + exact Hweak.
+    + apply IH.
+      * exact (proj2 Hweak).
+      * exact Hinh.
+Qed.
+
+Lemma point_in_hull_append_many_weak :
+  forall p suffix CH q,
+  weak_rev_ccw_list p (CH ++ suffix) ->
+  point_in_hull q (p :: CH) ->
+  point_in_hull q (p :: CH ++ suffix).
+Proof.
+  intros p suffix.
+  induction suffix as [| a suffix IH]; intros CH q Hweak Hinh.
+  - rewrite app_nil_r.
+    exact Hinh.
+  - assert (Hsnoc : weak_rev_ccw_list p (CH ++ [a])).
+    {
+      assert (Hfull : weak_rev_ccw_list p ((CH ++ [a]) ++ suffix ++ [])).
+      {
+        rewrite app_nil_r.
+        rewrite <- app_assoc.
+        simpl.
+        exact Hweak.
+      }
+      pose proof (weak_rev_ccw_list_remove_middle
+                    p (CH ++ [a]) suffix [] Hfull) as Htmp.
+      rewrite app_nil_r in Htmp.
+      exact Htmp.
+    }
+    assert (Hstep : point_in_hull q (p :: CH ++ [a])).
+    {
+      apply point_in_hull_snoc_weak.
+      - exact Hsnoc.
+      - exact Hinh.
+    }
+    replace (CH ++ a :: suffix) with ((CH ++ [a]) ++ suffix)
+      by (rewrite <- app_assoc; reflexivity).
+    apply IH.
+    + rewrite <- app_assoc.
+      simpl.
+      exact Hweak.
+    + exact Hstep.
+Qed.
+
+Lemma is_max_hull'_of_two_fans_weak :
+  forall p prefix joint suffix base,
+  weak_rev_ccw_list p (prefix ++ joint :: suffix) ->
+  Forall
+    (fun q =>
+       point_in_hull q (p :: prefix ++ [joint]) \/
+       point_in_hull q (p :: joint :: suffix))
+    base ->
+  is_max_hull' p (prefix ++ joint :: suffix) base.
+Proof.
+  intros p prefix joint suffix base Hweak Hcover.
+  unfold is_max_hull'.
+  rewrite Forall_forall in *.
+  intros q Hq.
+  specialize (Hcover q Hq) as [Hupper | Hlower].
+  - replace (prefix ++ joint :: suffix)
+      with ((prefix ++ [joint]) ++ suffix)
+      by (rewrite <- app_assoc; reflexivity).
+    apply point_in_hull_append_many_weak.
+    + rewrite <- app_assoc.
+      exact Hweak.
+    + exact Hupper.
+  - apply point_in_hull_prepend_many_weak.
+    + exact Hweak.
+    + exact Hlower.
+Qed.
+
+(** These are the two [point_in_hull] fans of the reversed merged tail
+    [first :: rev upper_mid ++ last :: rev lower_mid], not the raw semi-hull
+    paths.  The upper fan is the prefix ending at [last]; the lower fan starts
+    at [last] and then follows the reversed lower middle. *)
+Lemma andrew_two_fan_cover_to_merged_max_weak :
+  forall first last lower_mid upper_mid base,
+  weak_rev_ccw_list first (rev upper_mid ++ last :: rev lower_mid) ->
+  Forall
+    (fun q =>
+       point_in_hull q (first :: rev upper_mid ++ [last]) \/
+       point_in_hull q (first :: last :: rev lower_mid))
+    base ->
+  is_max_hull' first (rev upper_mid ++ last :: rev lower_mid) base.
+Proof.
+  intros first last lower_mid upper_mid base Hweak Hcover.
+  apply is_max_hull'_of_two_fans_weak.
+  - exact Hweak.
+  - exact Hcover.
+Qed.
+
+Lemma andrew_merged_triangle_max_of_two_fans :
+  forall first middle last lower_mid upper_mid,
+  leftmost first (lower_mid ++ last :: upper_mid) ->
+  ccw_convex (first :: lower_mid ++ last :: upper_mid) ->
+  Forall
+    (fun q =>
+       point_in_hull q (first :: rev upper_mid ++ [last]) \/
+       point_in_hull q (first :: last :: rev lower_mid))
+    (first :: middle ++ [last]) ->
+  is_max_hull' first (rev (lower_mid ++ last :: upper_mid))
+    (first :: middle ++ [last]).
+Proof.
+  intros first middle last lower_mid upper_mid Hleft Hconv Hcover.
+  simpl.
+  rewrite rev_app_distr.
+  simpl.
+  rewrite <- app_assoc.
+  simpl.
+  apply andrew_two_fan_cover_to_merged_max_weak.
+  - destruct (ccw_convex_tail_sort_rev
+                first (lower_mid ++ last :: upper_mid) Hleft Hconv)
+      as [_ Hweak].
+    simpl in Hweak.
+    rewrite rev_app_distr in Hweak.
+    simpl in Hweak.
+    rewrite <- app_assoc in Hweak.
+    simpl in Hweak.
+    exact Hweak.
+  - exact Hcover.
+Qed.
+
+Lemma weak_rev_ccw_list_lower_fan_from_merged_convex :
+  forall first lower_mid last upper_mid,
+  leftmost first (lower_mid ++ last :: upper_mid) ->
+  ccw_convex (first :: lower_mid ++ last :: upper_mid) ->
+  weak_rev_ccw_list first (last :: rev lower_mid).
+Proof.
+  intros first lower_mid last upper_mid Hleft Hconv.
+  destruct (ccw_convex_tail_sort_rev
+              first (lower_mid ++ last :: upper_mid) Hleft Hconv)
+    as [_ Hweak].
+  simpl in Hweak.
+  rewrite rev_app_distr in Hweak.
+  simpl in Hweak.
+  rewrite <- app_assoc in Hweak.
+  eapply (g_rev_ccw_list_ind' first (rev upper_mid)).
+  exact Hweak.
+Qed.
+
+Lemma lower_fan_covers_endpoints :
+  forall first lower_mid last upper_mid,
+  leftmost first (lower_mid ++ last :: upper_mid) ->
+  ccw_convex (first :: lower_mid ++ last :: upper_mid) ->
+  point_in_hull first (first :: last :: rev lower_mid) /\
+  point_in_hull last (first :: last :: rev lower_mid).
+Proof.
+  intros first lower_mid last upper_mid Hleft Hconv.
+  pose proof (weak_rev_ccw_list_lower_fan_from_merged_convex
+                first lower_mid last upper_mid Hleft Hconv) as Hweak.
+  split.
+  - apply gs_point_in_hull_anchor.
+    + discriminate.
+    + exact Hweak.
+  - apply gs_point_in_hull_new_head.
+    exact Hweak.
+Qed.
+
+Lemma andrew_two_fan_cover_of_middle :
+  forall first middle last lower_mid upper_mid,
+  leftmost first (lower_mid ++ last :: upper_mid) ->
+  ccw_convex (first :: lower_mid ++ last :: upper_mid) ->
+  Forall
+    (fun q =>
+       point_in_hull q (first :: rev upper_mid ++ [last]) \/
+       point_in_hull q (first :: last :: rev lower_mid))
+    middle ->
+  Forall
+    (fun q =>
+       point_in_hull q (first :: rev upper_mid ++ [last]) \/
+       point_in_hull q (first :: last :: rev lower_mid))
+    (first :: middle ++ [last]).
+Proof.
+  intros first middle last lower_mid upper_mid Hleft Hconv Hmiddle.
+  pose proof (lower_fan_covers_endpoints
+                first lower_mid last upper_mid Hleft Hconv)
+    as [Hfirst Hlast].
+  rewrite Forall_cons_iff.
+  split.
+  - right.
+    exact Hfirst.
+  - rewrite Forall_app.
+    split.
+    + exact Hmiddle.
+    + rewrite Forall_cons_iff.
+      split.
+      * right.
+        exact Hlast.
+      * apply Forall_nil.
+Qed.
+
+Lemma andrew_hull_max_from_middle_two_fan_cover :
+  forall first middle last lower_mid upper_mid,
+  point_xy_sorted (first :: middle ++ [last]) ->
+  (** coexisting head & last *)
+  andrew_lower_chain (first :: middle ++ [last]) =
+    first :: lower_mid ++ [last] ->
+  andrew_upper_chain (first :: middle ++ [last]) =
+    last :: upper_mid ++ [first] ->
+  (** semi-hull triangulation *)
+  Forall
+    (fun q =>
+       point_in_hull q (first :: rev upper_mid ++ [last]) \/
+       point_in_hull q (first :: last :: rev lower_mid))
+    middle ->
+  (** full-hull left-to-edges *)
+  is_max_hull'_edges
+    (andrew_hull (first :: middle ++ [last]))
+    (first :: middle ++ [last]).
+Proof.
+  intros first middle last lower_mid upper_mid
+    Hsorted Hlower Hupper Hmiddle.
+  assert (Hmerge :
+    andrew_ccw_merge
+      (first :: middle ++ [last])
+      (andrew_lower_chain (first :: middle ++ [last]))
+      (andrew_upper_chain (first :: middle ++ [last])) =
+      first :: lower_mid ++ last :: upper_mid).
+  {
+    eapply andrew_ccw_merge_endpoints; eauto.
+  }
+  assert (Hconv : ccw_convex (first :: lower_mid ++ last :: upper_mid)).
+  {
+    pose proof (andrew_hull_convex
+                  (first :: middle ++ [last]) Hsorted) as Hrevconv.
+    unfold andrew_hull, andrew_merge in Hrevconv.
+    rewrite Hmerge in Hrevconv.
+    apply gs_rev_ccw_convex_to_ccw_convex_rev in Hrevconv.
+    rewrite rev_involutive in Hrevconv.
+    exact Hrevconv.
+  }
+  assert (Hleft : leftmost first (lower_mid ++ last :: upper_mid)).
+  {
+    eapply andrew_ccw_merge_leftmost; eauto.
+  }
+  assert (Hcover :
+    Forall
+      (fun q =>
+         point_in_hull q (first :: rev upper_mid ++ [last]) \/
+         point_in_hull q (first :: last :: rev lower_mid))
+      (first :: middle ++ [last])).
+  {
+    eapply andrew_two_fan_cover_of_middle; eauto.
+  }
+  assert (Hmax :
+    is_max_hull' first (rev (lower_mid ++ last :: upper_mid))
+      (first :: middle ++ [last])).
+  {
+    eapply andrew_merged_triangle_max_of_two_fans; eauto.
+  }
+  eapply andrew_merged_triangle_max_to_edges; eauto.
+Qed.
+
+Lemma andrew_hull_max_f : forall sorted,
+  point_xy_sorted sorted ->
+  point_list_non_singleton sorted ->
+  is_max_hull'_edges (andrew_hull sorted) sorted.
+Proof.
+
+Abort.
+
+Theorem andrew_hull_max : forall sorted,
+  point_xy_sorted sorted ->
+  point_list_non_singleton sorted ->
+  is_max_hull'_edges (andrew_hull sorted) sorted.
+Proof.
+
+Abort.
+
+
+
+
+Definition andrew_hull_geometry_from_sorting (sorted : list point) : Prop :=
+  point_xy_sorted sorted ->
+  point_list_non_singleton sorted ->
+  andrew_hull_geometry sorted.
+
+Lemma andrew_hull_geometry_is_convex_hull : forall sorted T,
+  T = andrew_hull sorted ->
+  andrew_hull_geometry sorted ->
+  is_convex_hull sorted T.
+Proof.
+  intros sorted T HT Hgeom.
+  subst T.
+  exact (proj2 Hgeom).
+Qed.
